## Problem 6
![[Pasted image 20230425122809.png|800]]
**1)**
Assume that $u$ is a classical solution.
Multiply $u$ with $v$, and integrate gives:
$$-\int_{0}^{1}(a(x)u_{x})v \text{ d}x= \int_{0}^{1}1 \cdot v \text{ d}x$$
Integrating the LHS by parts:
$$-\left[a(x)u_{x}v \right]_{0}^{1} + \int _{0}^{1}a(x)u_{x}v_{x}\text{ d}x=\int_{0}^{1}v \text{ d}x$$
Calculating the boundary term:
$$(au_{x}v)(0)-(au_{x}v)(1) + \int _{0}^{1}a(x)u_{x}v_{x}\text{ d}x=\int_{0}^{1}v \text{ d}x$$
Note: we can **not** set $v(0)=v(1)=0$, since we then lose the Neumann BC. The Neumann BC gives that $u_{x}(0)=0$, but the second term is unknown. We want to throw away this term, so we add the condition the the function space $V$ that $v(1)=0$. Then the second term is zero. The equation becomes
$$\int _{0}^{1}a(x)u_{x}v_{x}\text{ d}x=\int_{0}^{1}v \text{ d}x-a(0)v(0).$$
Then the bilinear form and the linear functional becomes
$$a(u,v)=\int _{0}^{1}a(x)u_{x}v_{x}\text{ d}x$$
$$F(v)=\int_{0}^{1}v \text{ d}x-a(0)v(0).$$
**2) Space $V$**
Well defined if $u_{x},v_{x}, v \in L^{2}$
and $v(1)=0, v$ continuous in $x=0$.

$\implies\quad u,v \in V:= H^{1}_{\Gamma }(0,1)$
Where 
$$H^{1}_{\Gamma }=\{v \in H^{1}(0,1): \quad v(1)=0 \}$$
$\Gamma$ denotes where the Neumann conditions are. In this case $\Gamma =\{0 \}$

#### Observation
$V \subset H^{1}$,   $\lVert \cdot  \rVert_{V}=\lVert \cdot  \rVert_{H^1}$.
Some properties for $u,v \in H^{1}_{\Gamma }$

#### (a1) 
$a(u,v)$ is bilinear.

#### (a2)
$a(u,v)$ is continuous $\quad\implies\quad$ bounded on $H^{1}_{\Gamma }\times H^{1}_{\Gamma }$
Let's compute the bound
$$\begin{align*}
\lvert a(u,v) \rvert&\le  \int_{0}^{1}\lvert a(x) \rvert \cdot \lvert u_{x} \rvert \cdot \lvert v_{x}  \rvert \text{ d}x\\
		&\le \lVert a \rVert_{L^{\infty}} \int_{0}^{1}\lvert u_{x} \rvert \lvert v_{x} \rvert \text{ d}x\\
		&\stackrel{C.S}{\le} \lVert a \rVert_{L^{\infty}}\cdot \lVert u_{x} \rVert_{L^{2}} \cdot \lVert v_{x} \rVert_{L^{2}} \\
&\le \lVert a \rVert_{L^{\infty}}\cdot \lVert u_{x} \rVert_{H^{1}} \cdot \lVert v_{x} \rVert_{H^{1}}
\end{align*}$$
#### (a3)
$a(u,v)$ is **coercive**: 
Meaning that there is a positive lower bound for $a(u,u)$.
$$\begin{align*} a(u,u)&= \int_{0}^{1}a(x)u_{x}^{2}\text{ d}x \\ &\ge \min_\limits{x \in [0,1]}a(x)\int_{0}^{1}u_{x}^{2}\text{ d}x\\ &= :a_{0} \int _{0}^{1}u_{x}^{2}\text{ d}x \end{align*}$$
Where $a_{0}>0$ by assumtion.
	The Poincare inequality for $H^{1}_{\Gamma }$:
	$$\lVert u \rVert^{2}_{L^{2}}\le c \lVert u_{x} \rVert^{2}_{L^{2}}\quad\forall\quad u \in H^{1}_{\Gamma }$$
	$\implies\quad \lVert u \rVert^{2}_{H^{1}}=\lVert u \rVert^{2}_{L^{2}}+\lVert u_{x} \rVert^{2}_{L^{2}}\le (1+c) \lVert u_{x} \rVert^{2}_{L^{2}}$ 
Inserting this back gives 
$$a(u,u)\ge \frac{a_{0}}{1+c}\lVert u \rVert_{H^{1}}^{2}$$

Let's also check the linear functional 
#### (F1)
$F(v)$ linear
#### (F2)
$F(v)$ is bounded (=continuous) in $H^{1}_{\Gamma }$:
$$\begin{align*}
\lvert F(v) \rvert&\le  \int_{0}^{1}1 \cdot  \lvert v \rvert \text{ d}x+ \lvert v(0) \rvert \cdot \lvert a(0) \rvert\\
		&\le \lVert 1 \rVert_{L^{\infty}}\cdot \lVert v \rVert_{L^{\infty}} + \lVert v \rVert_{L^{\infty}} \cdot \lVert a \rVert_{L^{\infty}}\\
&\le  \lVert v \rVert_{L^{\infty}} + \lVert v_{x} \rVert_{L^{2}} \cdot \lVert a \rVert_{L^{\infty}}\\
	&\le (1 + \lVert a \rVert_{L^{\infty}})\cdot \lVert v \rVert_{H^{1}}
\end{align*}$$
Note that $v(x)=v(1)-\int_{x}^{1}v_{x} \text{ d}x= -\int_{x}^{1}v_{x} \text{ d}x$ so
$\max_\limits{x} \lvert v(x) \rvert=\max_\limits{x}\lvert \int_{x}^{1}v_{x} \text{ d}x \rvert$
$\le \max_\limits{x\int[0,1]} \int_{0}^{1}\lvert v_{x} \rvert\le \int_{0}^{1}\lvert v_{x} \rvert-1 \text{ d}x \le 1 \cdot \lVert v_{x} \rVert_{L^{2}}$

### Observation 2
Lax Milgram:
If
(a1) - (a3), (F1)-(F2), and $V$ a hilbert space, 
then
There exists a unique $u \in V = H^{1}_{\Gamma }\qquad\text{s.t.}\quad$
$$a(u,v)=F(v)= \quad\forall\quad v \in V.$$
![[Pasted image 20230425132006.png|800]]
Triangulation of space: 
$\mathcal{T}=\{I_{i} \}_{i=1}^{M},\quad I_{i}=(x_{i-1},x_{i})$
	Note: $\overline{\cup_{i}I_{i}}=[0,1]$.
	
$\mathbb{P}^{1}$ base functions:
#insert basis

$X^{1}_{h}:=\{v_{h}\in C[0,1]:\quad v_{h}|_{I_{i}} \text{ is linear } \quad\forall\quad i \}$
$=\text{span}\{\phi _{0},\dots,\phi _{M} \}$.

The space we use is
$V_{h}=X^{1}_{h}\cap H^{1}_{\Gamma }=\{v_{h}\in X^{1}_{h}:\quad v_{h}(1)=0 \}$
$=\text{span}\{\phi _{0},\dots,\phi _{M-1} \}$

**Observation**
	$u_{h}\in V_{h} \quad\Leftrightarrow\quad u_{h}(x)= \sum\limits_{j=0}^{M-1}U_{j}\phi _{j}(x)$
	for some $U_{j} \in \mathbb{R}$.

### Galerkin approximation
Find $u_{h}\in V_{h}$ $\left(\stackrel{u_{h}=\sum\limits_{}^{}U_{j}\phi _{j}}{\quad\Leftrightarrow\quad } \text{Find } U_{0},\dots ,U_{M-1}\right)$ such that
$$a(u_{h},v_{h})=F(v_{h})\quad\forall\quad v_{h}\in V_{h}$$
$$\Downarrow \quad \phi _{j} \text{ basis}$$
$$a(u_{h},\phi _{i})=F(\phi _{i}) \quad\text{for }i=0,\dots,M-1$$
$$\Downarrow \quad u_{h}=\sum\limits_{}^{}U_{j}\phi _{j}$$
$$\sum\limits_{j=0}^{M-1}a(\phi _{j},\phi _{i})U_{j}=F(\phi _{i}) \quad\text{for }i=0,\dots,M-1$$
$$\Downarrow$$
$$A \vec{U}=\vec{F}\tag{2}$$
where
$A_{ij}=a(\phi _{j},\phi _{i})$
$F_{i}=F(\phi _{i})$
$\vec{U}=[U_{0},\dots,U_{M-1}]^{T}$ 

#### Let $a(x)= \frac{1}{2}+x$,  find $A, \vec{F}$
$$A_{ij}=a(\phi _{j},\phi _{i})=\int_{0}^{1}\left( \frac{1}{2}+x\right) \phi _{j}'(x)\cdot \phi _{i}'(x)\text{ d}x$$
Obs: $\phi _{j}'(x) =\begin{cases} \frac{1}{h}  & \quad\text{for }x \in I_{j} \\ - \frac{1}{h} & \quad\text{for }x \in I_{j+1} \\0 & \quad \text{else} \end{cases}$
and $\phi _{0}'(x)=\begin{cases}- \frac{1}{h} & \quad\text{for }x \in (x_{0},x_{1}) \\0 & \text{else} \end{cases}$

Hence for $i=1,\dots,M-1$:
$$A_{ii}=\sum\limits_{k=1}^{M}\int_{I_{k}}\left( \frac{1}{2}+x\right)\phi _{i}' \phi _{i}' \text{ d}x$$
$$= 0 + \int_{x_{i-1}}^{x_{i}} \left( \frac{1}{2}+x\right) \left(\frac{1}{h} \right)^{2}\text{ d}x+ \int_{x_{i}}^{x_{i+1}}\left( \frac{1}{2}+x\right)\left(\frac{-1}{h} \right)^{2}$$
$$= \frac{1}{h^{2}}\int_{x_{i-1}}^{x_{i+1}} \left( \frac{1}{2}+x\right)\text{ d}x= \frac{1}{h^{2}}\left( \frac{1}{2}(x_{i+1}-x_{i-1}) + \frac{1}{2}(x_{i+1}^{2}-x_{i-1}^{2}) \right)$$
$$=\frac{1}{h^{2}} \left( \frac{1}{2}(x_{i+1}-x_{i-1}) + \frac{1}{2}(x_{i+1}+x_{i-1})(x_{i+1}-x_{i-1}) \right)$$
$$=\frac{1}{h^{2}} \left( \frac{1}{2}(2h) + \frac{1}{2}(2x_{i})(2h) \right) = \frac{1}{h}(1+2x_{i})$$
Now let's do $A_{i,i+1}$
$$A_{i,i+1}= 0+\dots+0+\int_{x_{i}}^{x_{i+1}}\left( \frac{1}{2}+x \right) \phi' _{i}\phi' _{i+1}\text{ d}x$$
$$=\int_{x_{i}}^{x_{i+1}}\left( \frac{1}{2}+x \right) \frac{1}{h} \cdot \frac{1}{-h} \text{ d}x$$
$$= \dots= - \frac{1}{2h}(1+2x_{i}+h)$$
Let's do $A_{i,i-1}$
$$A_{i,i-1}= \int _{x_{i-1}}^{x_{i}}\left( \frac{1}{2}+x \right) \frac{1}{h} \frac{1}{-h} \text{ d}x$$
$$= - \frac{1}{2} \frac{1}{h}(1+2x_{i}+h)$$

Last case: when $i=0$:
$$A_{00}= \frac{1}{h^{2}} \int_{0}^{h} \left( \frac{1}{2}+x\right)\text{ d}x= \frac{1}{2h}(1+h)$$
$A_{01}= - \frac{1}{h^{2}}\int_{0}^{h} \left( \frac{1}{2}+x \right)\text{ d}x=- \frac{1}{2h}(1+h)$

### Last part: find $F_{i}$
For $i=1,\dots,M-1$
$$F_{i}= \int _{0}^{1}1 \cdot \phi _{i}(x) \text{ d}x=\int _{x_{i-1}}^{x_{i+1}}\phi _{i}(x)\text{ d}x=\text{ Area of hat}= \frac{1}{2}2h \cdot 1=h$$
The boundaries:
$$\begin{align*}
F_{0}&= \int_{0}^{h} 1 \cdot \phi _{0}(x)\text{ d}x-a(0)\phi _{0}(0)\\
F_{0}&= \text{Area of hat}- \frac{1}{2}\cdot 1\\
&= \frac{1}{2}h \cdot 1- \frac{1}{2}= \frac{1}{2}(h-1)
\end{align*}$$
